\documentclass{article}

\usepackage{amsmath}

\begin{document}

\section{Solve the ODE}

\begin{align}
    {dr \over dt} &= u(1+z(1-{r(t) \over n}))-cr(t) \\
                  &= u(1+z)-r(t)(c+{uz \over n})
\end{align}

This is a linear ordinary differential equation and we know that $r(t)$ differentiates roughly into itself. So let's try a solution of the form $ae^{bt}$.

\begin{align}
             r(t) &= ae^{bt}+d \\
    {dr \over dt} &= bae^{bt} \\
                  &= b(r(t)-d) \\
                  &= br(t)-bd \\
       \implies b &= -(c+{uz \over n}) \\
               bd &= -u(1+z) \\
       \implies d &= {u(1+z) \over c+{uz \over n}} \\
    \implies r(t) &= ae^{-t(c+{uz \over n})}+{un(1+z) \over cn+uz}
\end{align}

Initial conditions give us

\begin{align}
             r(0) &= a+{un(1+z) \over cn+uz} \\
                a &= r(0)-{un(1+z) \over cn+uz} \\
    \implies r(t) &= (r(0)-{un(1+z) \over cn+uz})e^{-t(c+{uz \over n})}+{un(1+z) \over cn+uz}
\end{align}

\section{Differentiate the Solution}

Just in case.

\begin{align}
             r(t) &= (r(0)-{un(1+z) \over cn+uz})e^{-t(c+{uz \over n})}+{un(1+z) \over cn+uz} \\
    {dr \over dt} &= -(c+{uz \over n})(r(0)-{un(1+z) \over cn+uz})e^{-t(c+{uz \over n})} \\
                  &= -(c+{uz \over n})(r(t)-{un(1+z) \over cn+uz}) \\
                  &= u(1+z)-r(t)(c+{uz \over n})
\end{align}

\end{document}
